case_study/RiscvPmp/Contracts.v
@@ -39,6 +39,7 @@ From Katamaran Require Import
      Symbolic.Solver
      Symbolic.Propositions
      Symbolic.Worlds
+     RiscvPmp.PmpCheck
      RiscvPmp.Machine
      RiscvPmp.Sig.
 From Equations Require Import
