case_study/RiscvPmp/PmpCheck.v
@@ -1,0 +1,249 @@
+(******************************************************************************)
+(* Copyright (c) 2020 Steven Keuchel, Dominique Devriese, Sander Huyghebaert  *)
+(* All rights reserved.                                                       *)
+(*                                                                            *)
+(* Redistribution and use in source and binary forms, with or without         *)
+(* modification, are permitted provided that the following conditions are     *)
+(* met:                                                                       *)
+(*                                                                            *)
+(* 1. Redistributions of source code must retain the above copyright notice,  *)
+(*    this list of conditions and the following disclaimer.                   *)
+(*                                                                            *)
+(* 2. Redistributions in binary form must reproduce the above copyright       *)
+(*    notice, this list of conditions and the following disclaimer in the     *)
+(*    documentation and/or other materials provided with the distribution.    *)
+(*                                                                            *)
+(* THIS SOFTWARE IS PROVIDED BY THE COPYRIGHT HOLDERS AND CONTRIBUTORS        *)
+(* "AS IS" AND ANY EXPRESS OR IMPLIED WARRANTIES, INCLUDING, BUT NOT LIMITED  *)
+(* TO, THE IMPLIED WARRANTIES OF MERCHANTABILITY AND FITNESS FOR A PARTICULAR *)
+(* PURPOSE ARE DISCLAIMED. IN NO EVENT SHALL THE COPYRIGHT HOLDER OR          *)
+(* CONTRIBUTORS BE LIABLE FOR ANY DIRECT, INDIRECT, INCIDENTAL, SPECIAL,      *)
+(* EXEMPLARY, OR CONSEQUENTIAL DAMAGES (INCLUDING, BUT NOT LIMITED TO,        *)
+(* PROCUREMENT OF SUBSTITUTE GOODS OR SERVICES; LOSS OF USE, DATA, OR         *)
+(* PROFITS; OR BUSINESS INTERRUPTION) HOWEVER CAUSED AND ON ANY THEORY OF     *)
+(* LIABILITY, WHETHER IN CONTRACT, STRICT LIABILITY, OR TORT (INCLUDING       *)
+(* NEGLIGENCE OR OTHERWISE) ARISING IN ANY WAY OUT OF THE USE OF THIS         *)
+(* SOFTWARE, EVEN IF ADVISED OF THE POSSIBILITY OF SUCH DAMAGE.               *)
+(******************************************************************************)
+
+From Coq Require Import
+     ZArith.ZArith
+     Lists.List.
+From Katamaran Require Import
+     Bitvector
+     RiscvPmp.Base.
+
+Import ListNotations.
+Import bv.notations.
+
+Ltac bv_comp :=
+  repeat match goal with
+    | H: (?a <ᵘ? ?b) = true |- _ =>
+        rewrite bv.ultb_ult in H
+    | H: (?a <ᵘ? ?b) = false |- _ =>
+        rewrite bv.ultb_uge in H
+    | H: (?a <=ᵘ? ?b) = true |- _ =>
+        rewrite bv.uleb_ule in H
+    | H: (?a <=ᵘ? ?b) = false |- _ =>
+        rewrite bv.uleb_ugt in H
+    end.
+
+(* TODO: revert back to Iris/Stdpp rewrite tactic! (then remove tactic from Sig) *)
+Ltac bv_comp_bool :=
+  repeat match goal with
+    | H: ?a <ᵘ ?b |- _ =>
+        rewrite ? (proj2 (bv.ultb_ult _ _) H),
+                ? (proj2 (bv.uleb_ugt _ _) H);
+        clear H
+    | H: ?a <=ᵘ ?b |- _ =>
+        rewrite ? (proj2 (bv.uleb_ule _ _) H),
+                ? (proj2 (bv.ultb_uge _ _) H);
+        clear H
+    end.
+
+Definition PmpEntryCfg : Set := Pmpcfg_ent * Xlenbits.
+Definition PmpAddrRange := option (Xlenbits * Xlenbits).
+
+Definition pmp_addr_range (cfg : Pmpcfg_ent) (hi lo : Xlenbits) : PmpAddrRange :=
+  match A cfg with
+  | OFF => None
+  | TOR => Some (lo , hi)
+  end.
+
+Definition pmp_match_addr (a : Xlenbits) (width : Xlenbits) (rng : PmpAddrRange) : PmpAddrMatch :=
+  match rng with
+  | Some (lo, hi) =>
+      if hi <ᵘ? lo
+      then PMP_NoMatch
+      else if ((a + width <=ᵘ? lo)%bv || (hi <=ᵘ? a))%bool
+           then PMP_NoMatch
+           else if ((lo <=ᵘ? a) && (a + width <=ᵘ? hi)%bv)%bool
+                then PMP_Match
+                else PMP_PartialMatch
+  | None          => PMP_NoMatch
+  end.
+
+Definition pmp_match_entry (a width : Xlenbits) (m : Privilege) (cfg : Pmpcfg_ent) (lo hi : Xlenbits) : PmpMatch :=
+  let rng := pmp_addr_range cfg hi lo in
+  match pmp_match_addr a width rng with
+  | PMP_NoMatch      => PMP_Continue
+  | PMP_PartialMatch => PMP_Fail
+  | PMP_Match        => PMP_Success
+  end.
+
+Equations(noeqns) decide_access_pmp_perm (a : AccessType) (p : PmpCfgPerm) : bool :=
+| Read      | PmpR   := true;
+| Read      | PmpRW  := true;
+| Read      | PmpRX  := true;
+| Write     | PmpW   := true;
+| Write     | PmpRW  := true;
+| Write     | PmpWX  := true;
+| ReadWrite | PmpRW  := true;
+| Execute   | PmpX   := true;
+| Execute   | PmpRX  := true;
+| Execute   | PmpWX  := true;
+| _         | PmpRWX := true;
+| _         | _      := false.
+
+Definition pmp_get_RWX (cfg : Pmpcfg_ent) (p : Privilege) : PmpCfgPerm :=
+  match cfg with
+  | {| L := L; A := _; X := X; W := W; R := R |} =>
+      match L, p with
+      | false, Machine => PmpRWX
+      | _,     _       =>
+          match X, W, R with
+          | false, false, true  => PmpR
+          | false, true,  false => PmpW
+          | false, true,  true  => PmpRW
+          | true,  false, false => PmpX
+          | true,  false, true  => PmpRX
+          | true,  true,  false => PmpWX
+          | true,  true,  true  => PmpRWX
+          | _,     _,     _     => PmpO
+          end
+      end
+  end.
+
+Definition pmp_get_perms (cfg : Pmpcfg_ent) (p : Privilege) : PmpCfgPerm :=
+  match p with
+  | Machine =>
+      if L cfg
+      then pmp_get_RWX cfg p
+      else PmpRWX
+  | User =>
+      pmp_get_RWX cfg p
+  end.
+
+Fixpoint pmp_check_rec (n : nat) (a width lo : Xlenbits) (entries : list PmpEntryCfg) (p : Privilege) (acc : AccessType) : bool :=
+  match n, entries with
+  | S n, (cfg , hi) :: entries =>
+      match pmp_match_entry a width p cfg lo hi with
+      | PMP_Success  => decide_access_pmp_perm acc (pmp_get_perms cfg p)
+      | PMP_Fail     => false
+      | PMP_Continue => pmp_check_rec n a width hi entries p acc
+      end
+  | O, [] =>
+      match p with
+      | Machine => true
+      | _       => false
+      end
+  | _, _ => false
+  end%list.
+
+Definition pmp_check_aux (n : nat) (a width lo : Xlenbits) (entries : list PmpEntryCfg) (p : Privilege) (acc : AccessType) : bool :=
+  pmp_check_rec n a width lo entries p acc.
+
+Definition pmp_check (a width : Xlenbits) (entries : list PmpEntryCfg) (p : Privilege) (acc : AccessType) : bool :=
+  pmp_check_aux NumPmpEntries a width bv.zero entries p acc.
+
+Lemma addr_match_type_neq_off_cases :
+  forall a, a <> OFF -> a = TOR.
+Proof. now destruct a. Qed.
+
+Lemma addr_match_type_TOR_neq_OFF :
+  forall a, a = TOR -> a <> OFF.
+Proof. now destruct a. Qed.
+
+Lemma pmp_match_addr_match_conditions_1 : forall (paddr w lo hi : Xlenbits),
+    pmp_match_addr paddr w (Some (lo , hi)) = PMP_Match ->
+    lo <=ᵘ hi /\ lo <ᵘ (paddr + w)%bv /\ lo <=ᵘ paddr /\ paddr <ᵘ hi /\ (paddr + w)%bv <=ᵘ hi.
+Proof.
+  unfold pmp_match_addr.
+  intros paddr w lo hi H.
+  destruct (hi <ᵘ? lo) eqn:Ehilo; try discriminate H.
+  destruct ((paddr + w)%bv <=ᵘ? lo) eqn:Epwlo; first easy.
+  destruct (hi <=ᵘ? paddr) eqn:Ehip; first easy.
+  simpl in H.
+  destruct (lo <=ᵘ? paddr) eqn:Elop; last easy.
+  destruct ((paddr + w)%bv <=ᵘ? hi) eqn:Epwhi; last easy.
+  rewrite bv.ultb_antisym in Ehilo.
+  apply Bool.negb_false_iff in Ehilo.
+  now bv_comp.
+Qed.
+
+Lemma pmp_match_addr_match_conditions_2 : forall paddr w lo hi,
+    lo <=ᵘ hi ->
+    lo <ᵘ (paddr + w)%bv ->
+    lo <=ᵘ paddr ->
+    paddr <ᵘ hi ->
+    (paddr + w)%bv <=ᵘ hi ->
+    pmp_match_addr paddr w (Some (lo , hi)) = PMP_Match.
+Proof. intros; unfold pmp_match_addr; now bv_comp_bool. Qed.
+
+Lemma pmp_match_addr_nomatch_conditions : forall paddr w lo hi,
+    hi <ᵘ lo ->
+    pmp_match_addr paddr w (Some (lo , hi)) = PMP_NoMatch.
+Proof. intros; unfold pmp_match_addr; now bv_comp_bool. Qed.
+
+Lemma pmp_match_addr_nomatch_conditions_1 : forall paddr w lo hi,
+    (paddr + w)%bv <=ᵘ lo ->
+    pmp_match_addr paddr w (Some (lo , hi)) = PMP_NoMatch.
+Proof. intros; unfold pmp_match_addr; destruct (hi <ᵘ? lo); now bv_comp_bool. Qed.
+
+Lemma pmp_match_addr_nomatch_conditions_2 : forall paddr w lo hi,
+    hi <=ᵘ paddr ->
+    pmp_match_addr paddr w (Some (lo , hi)) = PMP_NoMatch.
+Proof.
+  intros.
+  unfold pmp_match_addr.
+  destruct (hi <ᵘ? lo) eqn:Ehilo; auto; bv_comp_bool.
+  now rewrite Bool.orb_true_r.
+Qed.
+
+Lemma pmp_match_addr_none: forall paddr w,
+    pmp_match_addr paddr w None = PMP_NoMatch.
+Proof. auto. Qed.
+
+Lemma pmp_match_addr_nomatch_1 : forall paddr w rng,
+    pmp_match_addr paddr w rng = PMP_NoMatch ->
+    rng = None \/
+      (forall lo hi, rng = Some (lo , hi) ->
+                (hi <ᵘ lo
+                 \/ (lo <=ᵘ hi /\ (paddr + w)%bv <=ᵘ lo)
+                 \/ (lo <=ᵘ hi /\ lo <ᵘ (paddr + w)%bv /\ hi <=ᵘ paddr))).
+Proof.
+  intros paddr w [[lo hi]|]; auto.
+  intros H.
+  right; intros l h Heq; inversion Heq; subst.
+  unfold pmp_match_addr in H.
+  destruct (h <ᵘ? l) eqn:?; bv_comp; auto.
+  destruct ((paddr + w)%bv <=ᵘ? l) eqn:?; bv_comp; simpl in H; auto.
+  destruct (h <=ᵘ? paddr) eqn:?; bv_comp; auto.
+  destruct (l <=ᵘ? paddr) eqn:?; destruct ((paddr + w)%bv <=ᵘ? h) eqn:?;
+    inversion H.
+Qed.
+
+Lemma pmp_match_addr_nomatch_2 : forall paddr w rng,
+    (rng = None \/
+       (forall lo hi, rng = Some (lo , hi) ->
+                 (hi <ᵘ lo \/ (paddr + w)%bv <=ᵘ lo \/ hi <=ᵘ paddr))) ->
+    pmp_match_addr paddr w rng = PMP_NoMatch.
+Proof.
+  intros paddr w [[lo hi]|]; auto.
+  intros [H|H].
+  inversion H.
+  destruct (H lo hi eq_refl) as [Hs|[Hs|Hs]]; revert Hs.
+  apply pmp_match_addr_nomatch_conditions.
+  apply pmp_match_addr_nomatch_conditions_1.
+  apply pmp_match_addr_nomatch_conditions_2.
+Qed.
